Revamp product type.
Now we distinguish public and oblivious product types which should be
conceptually cleaner. Most proofs are updated, but one proof in lifting
and demo are not done yet.

theories/lang_oadt/equivalence.v
@@ -52,11 +52,12 @@ Lemma pared_woval ω τ :
   woval τ.
 Proof.
   intros H. revert τ.
-  induction H; intros;
-    repeat match goal with
+  induction H; intros.
+  - repeat match goal with
            | H : ?e ⇛ _ |- _ => head_constructor e; sinvert H
            end; subst;
-    try case_split; eauto using woval.
+      try case_split; eauto using woval.
+  - econstructor. hauto use: pared_oval.
 Qed.
 
 (** ** Substitution lemmas *)
@@ -278,10 +279,10 @@ Proof.
   inv_solver.
 Qed.
 
-Lemma pared_inv_pair e1 e2 t :
-  <{ (e1, e2) }> ⇛ t ->
+Lemma pared_inv_pair l e1 e2 t :
+  <{ (e1, e2){l} }> ⇛ t ->
   exists e1' e2',
-    t = <{ (e1', e2') }> /\
+    t = <{ (e1', e2'){l} }> /\
     e1 ⇛ e1' /\
     e2 ⇛ e2'.
 Proof.
@@ -324,13 +325,16 @@ Ltac pared_intro_ e :=
 
 Ltac pared_intro :=
   match goal with
+  | |- <{ tape <{ ~if _ then _ else _ }> }> ⇛ _ => econstructor
+  | H : oval ?e |- <{ tape ?e }> ⇛ _ => eapply RTapeOVal
+  | |- <{ tape ?e }> ⇛ _ => eapply RCgrTape
   | |- ?e ⇛ _ => pared_intro_ e
   end.
 
 Ltac pared_inv_ e H :=
   match e with
   | <{ \:{_}_ => _ }> => apply pared_inv_abs in H; try simp_hyp H
-  | <{ (_, _) }> => apply pared_inv_pair in H; try simp_hyp H
+  | <{ (_, _){_} }> => apply pared_inv_pair in H; try simp_hyp H
   | <{ fold<_> _ }> => apply pared_inv_fold in H; try simp_hyp H
   | <{ inj@_<_> _ }> => apply pared_inv_inj in H; try simp_hyp H
   | _ => head_constructor e; sinvert H
@@ -368,7 +372,7 @@ Proof using Hwf.
   induction H; intros;
     (* Invert another parallel reduction. *)
     repeat pared_inv; simplify_eq;
-      try apply_gctx_wf; simplify_map_eq;
+      try oval_inv; try apply_gctx_wf; simplify_map_eq;
         (* Massage hypotheses related to oblivious values. *)
         try select! (oval _)
             (fun H => dup_hyp H (fun H => apply oval_lc in H));
@@ -391,7 +395,7 @@ Proof using Hwf.
                          end;
                      eauto; econstructor; eauto using lc, pared_lc2
            in try solve [ go
-                        (* First mung the induction hypotheses. *)
+                        (* First massage the induction hypotheses. *)
                         | repeat
                             match goal with
                             | H : forall _, _ ⇛ _ -> exists _, _ /\ _ |- _ =>
@@ -407,7 +411,7 @@ Proof using Hwf.
                       | _ ⇛ ?e =>
                         try assert (lc e) by eauto using pared_lc2
                       end);
-          (* Mung the induction hypotheses. *)
+          (* Massage the induction hypotheses. *)
           repeat
             match goal with
             | H : context [exists _, ?u ⇛ _ /\ _] |- _ =>
@@ -462,8 +466,8 @@ Proof using Hwf.
           | |- _ ∉ _ => shelve
           | |- lc _ =>
             eauto using lc, typing_lc, kinding_lc
-          | |- woval _ =>
-            eauto using pared_woval with lc
+          (* | |- woval _ => *)
+          (*   eauto using pared_woval with lc *)
           end
     in try case_split;
          try solve [ repeat esplit; cycle 1; repeat go; relax_pared; repeat go
@@ -489,8 +493,7 @@ Proof using Hwf.
     eauto; set_shelve.
 
   (* OADT application. *)
-  1-2:
-    repeat esplit; solve [ econstructor; eauto using lc ].
+  all: repeat esplit; solve [ econstructor; eauto using lc ].
 
   Unshelve.
   all : eauto; rewrite ?close_fv by eauto; fast_set_solver!!.
@@ -561,7 +564,7 @@ Inductive whnf : expr -> Prop :=
 | WUnitT : whnf <{ 𝟙 }>
 | WBool{l} : whnf <{ 𝔹{l} }>
 | WPi l τ1 τ2 : whnf <{ Π:{l}τ1, τ2 }>
-| WProd τ1 τ2 : whnf <{ τ1 * τ2 }>
+| WProd l τ1 τ2 : whnf <{ τ1 *{l} τ2 }>
 | WSum l τ1 τ2 : whnf <{ τ1 +{l} τ2 }>
 | WADT X τ :
     Σ !! X = Some (DADT τ) ->
@@ -577,10 +580,10 @@ Inductive whnf_equiv : expr -> expr -> Prop :=
     τ1 ≡ τ1' ->
     (forall x, x ∉ L -> <{ τ2^x }> ≡ <{ τ2'^x }>) ->
     whnf_equiv <{ Π:{l}τ1, τ2 }> <{ Π:{l}τ1', τ2' }>
-| WQProd τ1 τ2 τ1' τ2' :
+| WQProd l τ1 τ2 τ1' τ2' :
     τ1 ≡ τ1' ->
     τ2 ≡ τ2' ->
-    whnf_equiv <{ τ1 * τ2 }> <{ τ1' * τ2' }>
+    whnf_equiv <{ τ1 *{l} τ2 }> <{ τ1' *{l} τ2' }>
 | WQSum l τ1 τ2 τ1' τ2' :
     τ1 ≡ τ1' ->
     τ2 ≡ τ2' ->
@@ -773,13 +776,13 @@ Ltac congr_solver :=
     solve [ hauto ctrs: pared_equiv, pared use: pared_lc
           | induction H2; hauto ctrs: pared_equiv, pared use: pared_lc ].
 
-Lemma pared_equiv_congr_prod τ1 τ1' τ2 τ2' :
+Lemma pared_equiv_congr_prod τ1 τ1' τ2 τ2' l :
   τ1 ≡ τ1' ->
   τ2 ≡ τ2' ->
   lc τ1 ->
   lc τ2 ->
   lc τ2' ->
-  <{ τ1 * τ2 }> ≡ <{ τ1' * τ2' }>.
+  <{ τ1 *{l} τ2 }> ≡ <{ τ1' *{l} τ2' }>.
 Proof.
   congr_solver.
 Qed.
@@ -843,7 +846,7 @@ Ltac simpl_whnf_equiv :=
 Ltac apply_pared_equiv_congr :=
   lazymatch goal with
   | |- _ ⊢ Π:{_}_, _ ≡ Π:{_}_, _ => eapply pared_equiv_congr_pi
-  | |- _ ⊢ _ * _ ≡ _ * _ => eapply pared_equiv_congr_prod
+  | |- _ ⊢ _ *{_} _ ≡ _ *{_} _ => eapply pared_equiv_congr_prod
   | |- _ ⊢ _ +{_} _ ≡ _ +{_} _ => eapply pared_equiv_congr_sum
   | |- _ ⊢ inj{_}@_<_> _ ≡ inj{_}@_<_> _ => eapply pared_equiv_congr_inj
   end.
