theories/lang_oadt/semantics.v
@@ -7,28 +7,23 @@ Implicit Types (b : bool).
 
 (** ** Weak values *)
 Inductive wval : expr -> Prop :=
-| WUnitV : wval <{ () }>
 | WLit b : wval <{ lit b }>
 | WPair v1 v2 : wval v1 -> wval v2 -> wval <{ (v1, v2) }>
 | WAbs l τ e : wval <{ \:{l}τ => e }>
 | WInj b τ v : wval v -> wval <{ inj@b<τ> v }>
 | WFold X v : wval v -> wval <{ fold<X> v }>
-| WBoxedLit b : wval <{ [b] }>
-| WBoxedInj b ω v : otval ω -> oval v -> wval <{ [inj@b<ω> v] }>
 | WIte b v1 v2 :
     wval v1 -> wval v2 ->
     wval <{ ~if [b] then v1 else v2 }>
+| WOVal v : oval v -> wval v
 .
 
 (** ** Weak oblivious values *)
 Inductive woval : expr -> Prop :=
-| OWUnitV : woval <{ () }>
-| OWBoxedLit b : woval <{ [b] }>
-| OWPair v1 v2 : woval v1 -> woval v2 -> woval <{ (v1, v2) }>
-| OWBoxedInj b ω v : otval ω -> oval v -> woval <{ [inj@b<ω> v] }>
 | OWIte b v1 v2 :
     woval v1 -> woval v2 ->
     woval <{ ~if [b] then v1 else v2 }>
+| OWOVal v : oval v -> woval v
 .
 
 (** ** OADT value typing *)
@@ -40,7 +35,7 @@ Inductive ovalty : expr -> expr -> Prop :=
 | OTOBool b : ovalty <{ [b] }> <{ ~𝔹 }>
 | OTProd v1 v2 ω1 ω2 :
     ovalty v1 ω1 -> ovalty v2 ω2 ->
-    ovalty <{ (v1, v2) }> <{ ω1 * ω2 }>
+    ovalty <{ ~(v1, v2) }> <{ ω1 ~* ω2 }>
 | OTOSum b v ω1 ω2 :
     ovalty v <{ ite b ω1 ω2 }> ->
     (* Make sure the unused oblivious type is a value. *)
@@ -55,8 +50,8 @@ style later. This one can be quite annoying for proof automation. *)
 the hole in [ℇ] with [e]. [ectx ℇ] asserts that [ℇ] is a well-formed
 context. *)
 Variant ectx : (expr -> expr) -> Prop :=
-| CtxProd1 τ2 : ectx (fun τ1 => <{ τ1 * τ2 }>)
-| CtxProd2 ω1 : otval ω1 -> ectx (fun τ2 => <{ ω1 * τ2 }>)
+| CtxProd1 τ2 : ectx (fun τ1 => <{ τ1 ~* τ2 }>)
+| CtxProd2 ω1 : otval ω1 -> ectx (fun τ2 => <{ ω1 ~* τ2 }>)
 | CtxOSum1 τ2 : ectx (fun τ1 => <{ τ1 ~+ τ2 }>)
 | CtxOSum2 ω1 : otval ω1 -> ectx (fun τ2 => <{ ω1 ~+ τ2 }>)
 | CtxApp1 e2 : ectx (fun e1 => <{ e1 e2 }>)
@@ -68,9 +63,9 @@ Variant ectx : (expr -> expr) -> Prop :=
 | CtxOIte1 e1 e2 : ectx (fun e0 => <{ ~if e0 then e1 else e2 }>)
 | CtxOIte2 v0 e2 : wval v0 -> ectx (fun e1 => <{ ~if v0 then e1 else e2 }>)
 | CtxOIte3 v0 v1 : wval v0 -> wval v1 -> ectx (fun e2 => <{ ~if v0 then v1 else e2 }>)
-| CtxPair1 e2 : ectx (fun e1 => <{ (e1, e2) }>)
-| CtxPair2 v1 : wval v1 -> ectx (fun e2 => <{ (v1, e2) }>)
-| CtxProj b : ectx (fun e => <{ π@b e }>)
+| CtxPair1 l e2 : ectx (fun e1 => <{ (e1, e2){l} }>)
+| CtxPair2 l v1 : wval v1 -> ectx (fun e2 => <{ (v1, e2){l} }>)
+| CtxProj l b : ectx (fun e => <{ π{l}@b e }>)
 | CtxInj b τ : ectx (fun e => <{ inj@b<τ> e }>)
 | CtxOInj1 b e : ectx (fun τ => <{ ~inj@b<τ> e }>)
 | CtxOInj2 b ω : otval ω -> ectx (fun e => <{ ~inj@b<ω> e }>)
@@ -120,9 +115,9 @@ Inductive step : expr -> expr -> Prop :=
     <{ s𝔹 b }> -->! <{ [b] }>
 | SIte b e1 e2 :
     <{ if b then e1 else e2 }> -->! <{ ite b e1 e2 }>
-| SProj b v1 v2 :
+| SProj l b v1 v2 :
     wval v1 -> wval v2 ->
-    <{ π@b (v1, v2) }> -->! <{ ite b v1 v2 }>
+    <{ π{l}@b (v1, v2){l} }> -->! <{ ite b v1 v2 }>
 | SOInj b ω v :
     otval ω -> oval v ->
     <{ ~inj@b<ω> v }> -->! <{ [inj@b<ω> v] }>
@@ -144,18 +139,10 @@ Inductive step : expr -> expr -> Prop :=
 | STapeOIte b v1 v2 :
     woval v1 -> woval v2 ->
     <{ tape (~if [b] then v1 else v2) }> -->! <{ mux [b] (tape v1) (tape v2) }>
-| STapePair v1 v2 :
-    woval v1 -> woval v2 ->
-    <{ tape (v1, v2) }> -->! <{ (tape v1, tape v2) }>
-(* [tape v] is a no-op if [v] is an oblivious value (except for pair). Spell
-out all the cases here for determinism and proof convenience. *)
-| STapeUnitV :
-    <{ tape () }> -->! <{ () }>
-| STapeBoxedLit b :
-    <{ tape [b] }> -->! <{ [b] }>
-| STapeBoxedInj b ω v :
-    otval ω -> oval v ->
-    <{ tape [inj@b<ω> v] }> -->! <{ [inj@b<ω> v] }>
+(* [tape v] is a no-op if [v] is an oblivious value. *)
+| STapeOVal v :
+    oval v ->
+    <{ tape v }> -->! <{ v }>
 | SOIte b v1 v2 ℇ :
     lectx ℇ ->
     wval v1 -> wval v2 ->
