theories/lang_oadt/syntax.v
@@ -51,15 +51,18 @@ Inductive expr :=
 | ESec (e : expr)
 (* Public and oblivious conditional. The oblivious conditional may be leaky *)
 | EIte (l : olabel) (e0 e1 e2 : expr)
-(* Product *)
-| EProd (τ1 τ2 : expr)
-| EPair (e1 e2 : expr)
-| EProj (b : bool) (e : expr)
-(* Public and oblivious sum *)
+(* Public and oblivious product, pair and projection. Technically we do not need
+to distinguish bewteen public and oblivious product, but this is conceptually
+cleaner in my opinion. It also makes certain aspects of semantics and type
+checking more convenient. Note that the oblivious label can be easily inferred
+and elaborated, so the surface language needs not distinguish them. *)
+| EProd (l : olabel) (τ1 τ2 : expr)
+| EPair (l : olabel) (e1 e2 : expr)
+| EProj (l : olabel) (b : bool) (e : expr)
+(* Public and oblivious sum, injection and case analysis. The oblivious case may
+be leaky. *)
 | ESum (l : olabel) (τ1 τ2 : expr)
-(* Public and oblivious injection *)
 | EInj (l : olabel) (b : bool) (τ e : expr)
-(* Public and oblivious case. The oblivious case may be leaky *)
 | ECase (l : olabel) (e0 : expr) (e1 : expr) (e2 : expr)
 (* Introduction and elimination of ADTs *)
 | EFold (X : atom) (e : expr)
@@ -141,9 +144,17 @@ Notation "'𝔹'" := (EBool LPub) (in custom oadt at level 0).
 Notation "'Bool'" := (EBool LPub) (in custom oadt at level 0, only parsing).
 Notation "'~𝔹'" := (EBool LObliv) (in custom oadt at level 0).
 Notation "'~Bool'" := (EBool LObliv) (in custom oadt at level 0, only parsing).
-Notation "τ1 * τ2" := (EProd τ1 τ2) (in custom oadt at level 3,
-                                        τ1 custom oadt,
-                                        τ2 custom oadt at level 0).
+Notation "τ1 '*{' l '}' τ2" := (EProd l τ1 τ2) (in custom oadt at level 3,
+                                                   l constr at level 0,
+                                                   τ1 custom oadt,
+                                                   τ2 custom oadt at level 0,
+                                                  format "τ1  '*{' l '}'  τ2").
+Notation "τ1 * τ2" := (EProd LPub τ1 τ2) (in custom oadt at level 3,
+                                             τ1 custom oadt,
+                                             τ2 custom oadt at level 0).
+Notation "τ1 ~* τ2" := (EProd LObliv τ1 τ2) (in custom oadt at level 3,
+                                                τ1 custom oadt,
+                                                τ2 custom oadt at level 0).
 Notation "τ1 '+{' l '}' τ2" := (ESum l τ1 τ2) (in custom oadt at level 4,
                                                   l constr at level 0,
                                                   left associativity,
@@ -186,16 +197,38 @@ Notation "e1 e2" := (EApp e1 e2) (in custom oadt at level 2, left associativity)
 Notation "X @ e" := (ETApp X e) (in custom oadt at level 2,
                                     format "X @ e").
 Notation "()" := EUnitV (in custom oadt at level 0).
-Notation "( x , y , .. , z )" := (EPair .. (EPair x y) .. z)
+Notation "( x , y , .. , z ){ l }" := (EPair l .. (EPair l x y) .. z)
+                                        (in custom oadt at level 0,
+                                            l constr at level 0,
+                                            x custom oadt at level 99,
+                                            y custom oadt at level 99,
+                                            z custom oadt at level 99,
+                                            format "( x ,  y ,  .. ,  z ){ l }").
+Notation "( x , y , .. , z )" := (EPair LPub .. (EPair LPub x y) .. z)
                                    (in custom oadt at level 0,
                                        x custom oadt at level 99,
                                        y custom oadt at level 99,
                                        z custom oadt at level 99).
-Notation "'π@' b e" := (EProj b e) (in custom oadt at level 2,
-                                       b constr at level 0,
-                                       format "π@ b  e").
-Notation "'π1' e" := (EProj true e) (in custom oadt at level 2).
-Notation "'π2' e" := (EProj false e) (in custom oadt at level 2).
+Notation "~( x , y , .. , z )" := (EPair LObliv .. (EPair LObliv x y) .. z)
+                                    (in custom oadt at level 0,
+                                        x custom oadt at level 99,
+                                        y custom oadt at level 99,
+                                        z custom oadt at level 99,
+                                        format "~( x ,  y ,  .. ,  z )").
+Notation "'π{' l '}@' b e" := (EProj l b e) (in custom oadt at level 2,
+                                              l constr at level 0,
+                                              b constr at level 0,
+                                              format "π{ l }@ b  e").
+Notation "'π@' b e" := (EProj LPub b e) (in custom oadt at level 2,
+                                            b constr at level 0,
+                                            format "π@ b  e").
+Notation "'~π@' b e" := (EProj LObliv b e) (in custom oadt at level 2,
+                                               b constr at level 0,
+                                               format "~π@ b  e").
+Notation "'π1' e" := (EProj LPub true e) (in custom oadt at level 2).
+Notation "'π2' e" := (EProj LPub false e) (in custom oadt at level 2).
+Notation "'~π1' e" := (EProj LObliv true e) (in custom oadt at level 2).
+Notation "'~π2' e" := (EProj LObliv false e) (in custom oadt at level 2).
 Notation "'s𝔹' e" := (ESec e) (in custom oadt at level 2).
 Notation "'if{' l '}' e0 'then' e1 'else' e2" := (EIte l e0 e1 e2)
                                                    (in custom oadt at level 89,
@@ -336,9 +369,9 @@ Fixpoint open_ (k : nat) (s : expr) (e : expr) : expr :=
   | <{ X@e }> => <{ X@({k~>s}e) }>
   | <{ s𝔹 e }> => <{ s𝔹 ({k~>s}e) }>
   | <{ if{l} e0 then e1 else e2 }> => <{ if{l} {k~>s}e0 then {k~>s}e1 else {k~>s}e2 }>
-  | <{ τ1 * τ2 }> => <{ ({k~>s}τ1) * ({k~>s}τ2) }>
-  | <{ (e1, e2) }> => <{ ({k~>s}e1, {k~>s}e2) }>
-  | <{ π@b e }> => <{ π@b ({k~>s}e) }>
+  | <{ τ1 *{l} τ2 }> => <{ ({k~>s}τ1) *{l} ({k~>s}τ2) }>
+  | <{ (e1, e2){l} }> => <{ ({k~>s}e1, {k~>s}e2){l} }>
+  | <{ π{l}@b e }> => <{ π{l}@b ({k~>s}e) }>
   | <{ τ1 +{l} τ2 }> => <{ ({k~>s}τ1) +{l} ({k~>s}τ2) }>
   | <{ inj{l}@b<τ> e }> => <{ inj{l}@b<({k~>s}τ)> ({k~>s}e) }>
   | <{ fold<X> e }> => <{ fold<X> ({k~>s}e) }>
@@ -367,9 +400,9 @@ Fixpoint subst (x : atom) (s : expr) (e : expr) : expr :=
   | <{ let e1 in e2 }> => <{ let {x↦s}e1 in {x↦s}e2 }>
   | <{ s𝔹 e }> => <{ s𝔹 ({x↦s}e) }>
   | <{ if{l} e0 then e1 else e2 }> => <{ if{l} {x↦s}e0 then {x↦s}e1 else {x↦s}e2 }>
-  | <{ τ1 * τ2 }> => <{ ({x↦s}τ1) * ({x↦s}τ2) }>
-  | <{ (e1, e2) }> => <{ ({x↦s}e1, {x↦s}e2) }>
-  | <{ π@b e }> => <{ π@b ({x↦s}e) }>
+  | <{ τ1 *{l} τ2 }> => <{ ({x↦s}τ1) *{l} ({x↦s}τ2) }>
+  | <{ (e1, e2){l} }> => <{ ({x↦s}e1, {x↦s}e2){l} }>
+  | <{ π{l}@b e }> => <{ π{l}@b ({x↦s}e) }>
   | <{ τ1 +{l} τ2 }> => <{ ({x↦s}τ1) +{l} ({x↦s}τ2) }>
   | <{ inj{l}@b<τ> e }> => <{ inj{l}@b<({x↦s}τ)> ({x↦s}e) }>
   | <{ case{l} e0 of e1 | e2 }> => <{ case{l} {x↦s}e0 of {x↦s}e1 | {x↦s}e2 }>
@@ -388,7 +421,7 @@ Definition lexpr_subst x s (T : lexpr) := (T.1, subst x s T.2).
 Inductive otval : expr -> Prop :=
 | OVUnitT : otval <{ 𝟙 }>
 | OVOBool : otval <{ ~𝔹 }>
-| OVProd ω1 ω2 : otval ω1 -> otval ω2 -> otval <{ ω1 * ω2 }>
+| OVProd ω1 ω2 : otval ω1 -> otval ω2 -> otval <{ ω1 ~* ω2 }>
 | OVOSum ω1 ω2 : otval ω1 -> otval ω2 -> otval <{ ω1 ~+ ω2 }>
 .
 
@@ -396,20 +429,18 @@ Inductive otval : expr -> Prop :=
 Inductive oval : expr -> Prop :=
 | OVUnitV : oval <{ () }>
 | OVBoxedLit b : oval <{ [b] }>
-| OVPair v1 v2 : oval v1 -> oval v2 -> oval <{ (v1, v2) }>
+| OVPair v1 v2 : oval v1 -> oval v2 -> oval <{ ~(v1, v2) }>
 | OVBoxedInj b ω v : otval ω -> oval v -> oval <{ [inj@b<ω> v] }>
 .
 
 (** ** Values (v) *)
 Inductive val : expr -> Prop :=
-| VUnitV : val <{ () }>
 | VLit b : val <{ lit b }>
 | VPair v1 v2 : val v1 -> val v2 -> val <{ (v1, v2) }>
 | VAbs l τ e : val <{ \:{l}τ => e }>
 | VInj b τ v : val v -> val <{ inj@b<τ> v }>
 | VFold X v : val v -> val <{ fold<X> v }>
-| VBoxedLit b : val <{ [b] }>
-| VBoxedInj b ω v : otval ω -> oval v -> val <{ [inj@b<ω> v] }>
+| VOVal v : oval v -> val v
 .
 
 (** ** Local closure and well-formedness of expressions *)
@@ -438,9 +469,9 @@ Inductive lc : expr -> Prop :=
 | LCLit b : lc <{ lit b }>
 | LCSec e : lc e -> lc <{ s𝔹 e }>
 | LCIte l e0 e1 e2 : lc e0 -> lc e1 -> lc e2 -> lc <{ if{l} e0 then e1 else e2 }>
-| LCProd τ1 τ2 : lc τ1 -> lc τ2 -> lc <{ τ1 * τ2 }>
-| LCPair e1 e2 : lc e1 -> lc e2 -> lc <{ (e1, e2) }>
-| LCProj b e : lc e -> lc <{ π@b e }>
+| LCProd l τ1 τ2 : lc τ1 -> lc τ2 -> lc <{ τ1 *{l} τ2 }>
+| LCPair l e1 e2 : lc e1 -> lc e2 -> lc <{ (e1, e2){l} }>
+| LCProj l b e : lc e -> lc <{ π{l}@b e }>
 | LCSum l τ1 τ2 : lc τ1 -> lc τ2 -> lc <{ τ1 +{l} τ2 }>
 | LCInj l b τ e : lc τ -> lc e -> lc <{ inj{l}@b<τ> e }>
 | LCFold X e : lc e -> lc <{ fold<X> e }>
