theories/lang_oadt/dec.v
@@ -1,5 +1,6 @@
 (** Some decision procedures and implementations. *)
-From oadt.lang_oadt Require Import base syntax semantics infrastructure admissible.
+From oadt.lang_oadt Require Import
+     base syntax semantics infrastructure admissible values.
 Import syntax.notations semantics.notations.
 
 (** * Decision procedures *)
@@ -9,8 +10,10 @@ Section dec.
 within Coq. *)
 Ltac t :=
   solve [ repeat
-            (try solve [ left; abstract (econstructor; assumption)
-                       | right; abstract (inversion 1; subst; contradiction) ];
+            (try solve [ left; abstract (econstructor; eauto using oval)
+                       | right; abstract (inversion 1; subst;
+                                          try contradiction;
+                                          repeat oval_inv) ];
              try match reverse goal with
                  | H : sumbool _ _ |- _ => destruct H
                  end) ].
@@ -24,7 +27,7 @@ Defined.
 #[global]
 Instance oval_dec v : Decision (oval v).
 Proof.
-  hnf. induction v; try t.
+  hnf. induction v; try t; try case_label; try t.
 
   match goal with
   | H : context [ oval ?ω ] |- context [<{ [inj@_<(?ω)> _] }>] =>
@@ -36,16 +39,14 @@ Defined.
 Instance wval_dec v : Decision (wval v).
 Proof.
   hnf. induction v; try t; try case_label; try t.
-  - match goal with
-    | H : context [ wval ?v] |- context [<{ ~if ?v then _ else _ }>] =>
+  match goal with
+  | H : context [ wval ?v] |- context [<{ ~if ?v then _ else _ }>] =>
       clear H; destruct v; try t
-    end.
-  - match goal with
-    | H : context [ wval ?ω], H' : context [ wval ?v ] |-
-      context [<{ [inj@_<(?ω)> ?v] }>] =>
-      clear H; clear H';
-        destruct (decide (otval ω)); try t;
-        destruct (decide (oval v)); try t
+  end.
+  all:
+    match goal with
+    | |- context [ wval ?e ] =>
+        destruct (decide (oval e)); t
     end.
 Defined.
 
@@ -53,16 +54,14 @@ Defined.
 Instance woval_dec v : Decision (woval v).
 Proof.
   hnf. induction v; try t; try case_label; try t.
-  - match goal with
-    | H : context [ woval ?v] |- context [<{ ~if ?v then _ else _ }>] =>
+  match goal with
+  | H : context [ woval ?v] |- context [<{ ~if ?v then _ else _ }>] =>
       clear H; destruct v; try t
-    end.
-  - match goal with
-    | H : context [ woval ?ω], H' : context [ woval ?v ] |-
-      context [<{ [inj@_<(?ω)> ?v] }>] =>
-      clear H; clear H';
-        destruct (decide (otval ω)); try t;
-        destruct (decide (oval v)); try t
+  end.
+  all:
+    match goal with
+    | |- context [ woval ?e ] =>
+        destruct (decide (oval e)); t
     end.
 Defined.
 
@@ -70,13 +69,11 @@ Defined.
 Instance val_dec v : Decision (val v).
 Proof.
   hnf. induction v; try t; try case_label; try t.
-  match goal with
-  | H : context [ val ?ω], H' : context [ val ?v ] |-
-      context [<{ [inj@_<(?ω)> ?v] }>] =>
-      clear H; clear H';
-      destruct (decide (otval ω)); try t;
-      destruct (decide (oval v)); try t
-  end.
+  all:
+    match goal with
+    | |- context [ val ?e ] =>
+        destruct (decide (oval e)); t
+    end.
 Defined.
 
 End dec.
@@ -94,7 +91,7 @@ Fixpoint ovalty_ (ω : expr) : option expr :=
   match ω with
   | <{ 𝟙 }> => mret <{ () }>
   | <{ ~𝔹 }> => mret <{ [true] }>
-  | <{ ω1 * ω2 }> => v1 <- ovalty_ ω1; v2 <- ovalty_ ω2; mret <{ (v1, v2) }>
+  | <{ ω1 ~* ω2 }> => v1 <- ovalty_ ω1; v2 <- ovalty_ ω2; mret <{ ~(v1, v2) }>
   | <{ ω1 ~+ ω2 }> =>
       guard (otval ω2); v <- ovalty_ ω1; mret <{ [inl<ω1 ~+ ω2> v] }>
   | _ => None
@@ -148,14 +145,14 @@ Fixpoint step_ (e : expr) : option expr :=
          | _ => None
          end
     else e0' <- step_ e0; mret <{ if e0' then e1 else e2 }>
-  | <{ τ1 * τ2 }> =>
+  | <{ τ1 ~* τ2 }> =>
     if decide (otval τ1)
-    then τ2' <- step_ τ2; mret <{ τ1 * τ2' }>
-    else τ1' <- step_ τ1; mret <{ τ1' * τ2 }>
-  | <{ (e1, e2) }> =>
+    then τ2' <- step_ τ2; mret <{ τ1 ~* τ2' }>
+    else τ1' <- step_ τ1; mret <{ τ1' ~* τ2 }>
+  | <{ (e1, e2){l} }> =>
     if decide (wval e1)
-    then e2' <- step_ e2; mret <{ (e1, e2') }>
-    else e1' <- step_ e1; mret <{ (e1', e2) }>
+    then e2' <- step_ e2; mret <{ (e1, e2'){l} }>
+    else e1' <- step_ e1; mret <{ (e1', e2){l} }>
   | <{ π@b e }> =>
     if decide (wval e)
     then match e with
@@ -165,6 +162,13 @@ Fixpoint step_ (e : expr) : option expr :=
          | _ => None
          end
     else e' <- step_ e; mret <{ π@b e' }>
+  | <{ ~π@b e }> =>
+    if decide (wval e)
+    then match e with
+         | <{ ~(v1, v2) }> => mret <{ ite b v1 v2 }>
+         | _ => None
+         end
+    else e' <- step_ e; mret <{ ~π@b e' }>
   | <{ τ1 ~+ τ2 }> =>
     if decide (otval τ1)
     then τ2' <- step_ τ2; mret <{ τ1 ~+ τ2' }>
@@ -210,12 +214,7 @@ Fixpoint step_ (e : expr) : option expr :=
     then match e with
          | <{ ~if [b] then v1 else v2 }> =>
            mret <{ mux [b] (tape v1) (tape v2) }>
-         | <{ (v1, v2) }> =>
-           mret <{ (tape v1, tape v2) }>
-         | <{ () }> => mret <{ () }>
-         | <{ [b] }> => mret <{ [b] }>
-         | <{ [inj@b<ω> v] }> => mret <{ [inj@b<ω> v] }>
-         | _ => None
+         | _ => mret e
          end
     else e' <- step_ e; mret <{ tape e' }>
   | <{ mux e0 e1 e2 }> =>
@@ -272,7 +271,7 @@ Proof.
       match goal with
       | H : match ?e with _ => _ end = _ |- _ =>
           sdestruct e; simplify_eq
-      end; try wval_inv; try woval_inv;
+      end; try wval_inv; try woval_inv; try oval_inv;
     (* Remove induction hypotheses when they are not needed to avoid unnecessary
     subgoals from [simplify_option_eq]. *)
     repeat
@@ -281,7 +280,7 @@ Proof.
           assert_fails is_var e; clear IH
       end;
     simplify_option_eq;
-    try solve [ eauto using step | solve_ctx ].
+    try solve [ eauto using step, oval, oval_wval | solve_ctx ].
 
   eauto using step, ovalty_sound.
 Qed.
